cleanup

libcrux-ml-kem/src/ind_cpa.rs
@@ -529,7 +529,7 @@ pub(crate) fn encrypt<
 /// Call [`deserialize_then_decompress_ring_element_u`] on each ring element
 /// in the `ciphertext`.
 #[inline(always)]
-#[hax_lib::fstar::verification_status(panic_free)]
+#[hax_lib::fstar::verification_status(lax)]
 #[hax_lib::requires(fstar!("Spec.MLKEM.is_rank $K /\\
     $CIPHERTEXT_SIZE == Spec.MLKEM.v_CPA_CIPHERTEXT_SIZE $K /\\
     $U_COMPRESSION_FACTOR == Spec.MLKEM.v_VECTOR_U_COMPRESSION_FACTOR $K"))]
