libcrux-ml-kem/src/vector/avx2.rs
@@ -18,7 +18,7 @@ pub struct SIMD256Vector {
 #[inline(always)]
 #[hax_lib::fstar::verification_status(panic_free)]
 #[hax_lib::ensures(|result| fstar!("repr ${result} == Seq.create 16 0s"))]
-fn zero() -> SIMD256Vector {
+fn vec_zero() -> SIMD256Vector {
     SIMD256Vector {
         elements: mm256_setzero_si256(),
     }
@@ -28,7 +28,7 @@ fn zero() -> SIMD256Vector {
 #[inline(always)]
 #[hax_lib::fstar::verification_status(panic_free)]
 #[hax_lib::ensures(|result| fstar!("${result} == repr ${v}"))]
-fn to_i16_array(v: SIMD256Vector) -> [i16; 16] {
+fn vec_to_i16_array(v: SIMD256Vector) -> [i16; 16] {
     let mut output = [0i16; 16];
     mm256_storeu_si256_i16(&mut output, v.elements);
 
@@ -38,7 +38,7 @@ fn to_i16_array(v: SIMD256Vector) -> [i16; 16] {
 #[inline(always)]
 #[hax_lib::fstar::verification_status(panic_free)]
 #[hax_lib::ensures(|result| fstar!("repr ${result} == ${array}"))]
-fn from_i16_array(array: &[i16]) -> SIMD256Vector {
+fn vec_from_i16_array(array: &[i16]) -> SIMD256Vector {
     SIMD256Vector {
         elements: mm256_loadu_si256_i16(array),
     }
@@ -46,7 +46,7 @@ fn from_i16_array(array: &[i16]) -> SIMD256Vector {
 
 impl Repr for SIMD256Vector {
     fn repr(x: Self) -> [i16; 16] {
-        to_i16_array(x)
+        vec_to_i16_array(x)
     }
 }
 
@@ -54,18 +54,18 @@ impl Repr for SIMD256Vector {
 impl Operations for SIMD256Vector {
     #[ensures(|result| fstar!("impl.f_repr out == Seq.create 16 0s"))]
     fn ZERO() -> Self {
-        zero()
+        vec_zero()
     }
 
     #[requires(array.len() == 16)]
     #[ensures(|result| fstar!("impl.f_repr out == $array"))]
     fn from_i16_array(array: &[i16]) -> Self {
-        from_i16_array(array)
+        vec_from_i16_array(array)
     }
 
     #[ensures(|result| fstar!("out == impl.f_repr $x"))]
     fn to_i16_array(x: Self) -> [i16; 16] {
-        to_i16_array(x)
+        vec_to_i16_array(x)
     }
 
     #[ensures(|result| fstar!("impl.f_repr out == Spec.Utils.map2 (+.) (impl.f_repr $lhs) (impl.f_repr $rhs)"))]
