libcrux-ml-kem/proofs/fstar/extraction/Libcrux_ml_kem.Vector.Avx2.fst
@@ -9,14 +9,14 @@ let _ =
   let open Libcrux_ml_kem.Vector.Traits in
   ()
 
-let from_i16_array (array: t_Slice i16) =
+let vec_from_i16_array (array: t_Slice i16) =
   let result:t_SIMD256Vector =
     { f_elements = Libcrux_intrinsics.Avx2_extract.mm256_loadu_si256_i16 array } <: t_SIMD256Vector
   in
   let _:Prims.unit = admit () (* Panic freedom *) in
   result
 
-let to_i16_array (v: t_SIMD256Vector) =
+let vec_to_i16_array (v: t_SIMD256Vector) =
   let output:t_Array i16 (sz 16) = Rust_primitives.Hax.repeat 0s (sz 16) in
   let output:t_Array i16 (sz 16) =
     Libcrux_intrinsics.Avx2_extract.mm256_storeu_si256_i16 output v.f_elements
@@ -25,7 +25,7 @@ let to_i16_array (v: t_SIMD256Vector) =
   let _:Prims.unit = admit () (* Panic freedom *) in
   result
 
-let zero (_: Prims.unit) =
+let vec_zero (_: Prims.unit) =
   let result:t_SIMD256Vector =
     { f_elements = Libcrux_intrinsics.Avx2_extract.mm256_setzero_si256 () } <: t_SIMD256Vector
   in
