libcrux-ml-kem/proofs/fstar/extraction/Libcrux_ml_kem.Vector.Avx2.fsti
@@ -15,7 +15,7 @@ type t_SIMD256Vector = { f_elements:Libcrux_intrinsics.Avx2_extract.t_Vec256 }
 
 let repr (x:t_SIMD256Vector) : t_Array i16 (sz 16) = Libcrux_intrinsics.Avx2_extract.vec256_as_i16x16 x.f_elements
 
-val from_i16_array (array: t_Slice i16)
+val vec_from_i16_array (array: t_Slice i16)
     : Prims.Pure t_SIMD256Vector
       Prims.l_True
       (ensures
@@ -23,7 +23,7 @@ val from_i16_array (array: t_Slice i16)
           let result:t_SIMD256Vector = result in
           repr result == array)
 
-val to_i16_array (v: t_SIMD256Vector)
+val vec_to_i16_array (v: t_SIMD256Vector)
     : Prims.Pure (t_Array i16 (sz 16))
       Prims.l_True
       (ensures
@@ -38,10 +38,10 @@ let impl: Libcrux_ml_kem.Vector.Traits.t_Repr t_SIMD256Vector =
     _super_9442900250278684536 = FStar.Tactics.Typeclasses.solve;
     f_repr_pre = (fun (x: t_SIMD256Vector) -> true);
     f_repr_post = (fun (x: t_SIMD256Vector) (out: t_Array i16 (sz 16)) -> true);
-    f_repr = fun (x: t_SIMD256Vector) -> to_i16_array x
+    f_repr = fun (x: t_SIMD256Vector) -> vec_to_i16_array x
   }
 
-val zero: Prims.unit
+val vec_zero: Prims.unit
   -> Prims.Pure t_SIMD256Vector
       Prims.l_True
       (ensures
@@ -59,19 +59,19 @@ let impl_3: Libcrux_ml_kem.Vector.Traits.t_Operations t_SIMD256Vector =
     f_ZERO_post
     =
     (fun (_: Prims.unit) (out: t_SIMD256Vector) -> impl.f_repr out == Seq.create 16 0s);
-    f_ZERO = (fun (_: Prims.unit) -> zero ());
+    f_ZERO = (fun (_: Prims.unit) -> vec_zero ());
     f_from_i16_array_pre
     =
     (fun (array: t_Slice i16) -> (Core.Slice.impl__len #i16 array <: usize) =. sz 16);
     f_from_i16_array_post
     =
     (fun (array: t_Slice i16) (out: t_SIMD256Vector) -> impl.f_repr out == array);
-    f_from_i16_array = (fun (array: t_Slice i16) -> from_i16_array array);
+    f_from_i16_array = (fun (array: t_Slice i16) -> vec_from_i16_array array);
     f_to_i16_array_pre = (fun (x: t_SIMD256Vector) -> true);
     f_to_i16_array_post
     =
     (fun (x: t_SIMD256Vector) (out: t_Array i16 (sz 16)) -> out == impl.f_repr x);
-    f_to_i16_array = (fun (x: t_SIMD256Vector) -> to_i16_array x);
+    f_to_i16_array = (fun (x: t_SIMD256Vector) -> vec_to_i16_array x);
     f_add_pre = (fun (lhs: t_SIMD256Vector) (rhs: t_SIMD256Vector) -> true);
     f_add_post
     =
